code/ecdsap256/Hacl.Impl.P256.Point.fsti
@@ -17,18 +17,7 @@ module SM = Hacl.Spec.P256.MontgomeryMultiplication
 
 #set-options "--z3rlimit 30 --fuel 0 --ifuel 0"
 
-inline_for_extraction noextract
-let point_seq = LSeq.lseq uint64 12
-
-let as_point_nat_seq (p:point_seq) =
-  felem_seq_as_nat (LSeq.sub p 0 4),
-  felem_seq_as_nat (LSeq.sub p 4 4),
-  felem_seq_as_nat (LSeq.sub p 8 4)
-
-let point_inv_seq (p:point_seq) =
-  let x, y, z = as_point_nat_seq p in
-  x < S.prime /\ y < S.prime /\ z < S.prime
-
+///  Affine coordinates
 
 inline_for_extraction noextract
 let aff_point_seq = LSeq.lseq uint64 8
@@ -41,6 +30,52 @@ let aff_point_inv_seq (p:aff_point_seq) =
   let x, y = as_aff_point_nat_seq p in
   x < S.prime /\ y < S.prime
 
+
+inline_for_extraction noextract
+let aff_point = lbuffer uint64 8ul
+
+noextract
+let as_aff_point_nat (h:mem) (p:aff_point) =
+  as_aff_point_nat_seq (as_seq h p)
+
+noextract
+let aff_point_inv (h:mem) (p:aff_point) =
+  aff_point_inv_seq (as_seq h p)
+
+noextract
+let aff_point_x_as_nat (h:mem) (p:aff_point) : GTot nat =
+  as_nat h (gsub p 0ul 4ul)
+
+noextract
+let aff_point_y_as_nat (h:mem) (p:aff_point) : GTot nat =
+  as_nat h (gsub p 4ul 4ul)
+
+inline_for_extraction noextract
+let aff_getx (p:aff_point) : Stack felem
+  (requires fun h -> live h p)
+  (ensures fun h0 f h1 -> f == gsub p 0ul 4ul /\ h0 == h1)
+  = sub p 0ul 4ul
+
+inline_for_extraction noextract
+let aff_gety (p:aff_point) : Stack felem
+  (requires fun h -> live h p)
+  (ensures fun h0 f h1 -> f == gsub p 4ul 4ul /\ h0 == h1)
+  = sub p 4ul 4ul
+
+
+///  Jacobian coordinates
+
+inline_for_extraction noextract
+let point_seq = LSeq.lseq uint64 12
+
+let as_point_nat_seq (p:point_seq) =
+  felem_seq_as_nat (LSeq.sub p 0 4),
+  felem_seq_as_nat (LSeq.sub p 4 4),
+  felem_seq_as_nat (LSeq.sub p 8 4)
+
+let point_inv_seq (p:point_seq) =
+  let x, y, z = as_point_nat_seq p in
+  x < S.prime /\ y < S.prime /\ z < S.prime
 
 
 inline_for_extraction noextract
@@ -86,57 +121,25 @@ let getz (p:point) : Stack felem
   = sub p 8ul 4ul
 
 
-inline_for_extraction noextract
-let aff_point = lbuffer uint64 8ul
-
-noextract
-let as_aff_point_nat (h:mem) (p:aff_point) =
-  as_aff_point_nat_seq (as_seq h p)
-
-noextract
-let aff_point_inv (h:mem) (p:aff_point) =
-  aff_point_inv_seq (as_seq h p)
-
-noextract
-let aff_point_x_as_nat (h:mem) (p:aff_point) : GTot nat =
-  as_nat h (gsub p 0ul 4ul)
-
-noextract
-let aff_point_y_as_nat (h:mem) (p:aff_point) : GTot nat =
-  as_nat h (gsub p 4ul 4ul)
+///  Create a point
 
 inline_for_extraction noextract
-let aff_getx (p:aff_point) : Stack felem
-  (requires fun h -> live h p)
-  (ensures fun h0 f h1 -> f == gsub p 0ul 4ul /\ h0 == h1)
-  = sub p 0ul 4ul
-
-inline_for_extraction noextract
-let aff_gety (p:aff_point) : Stack felem
-  (requires fun h -> live h p)
-  (ensures fun h0 f h1 -> f == gsub p 4ul 4ul /\ h0 == h1)
-  = sub p 4ul 4ul
-
+val create_point: unit -> StackInline point
+  (requires fun h -> True)
+  (ensures  fun h0 f h1 ->
+    stack_allocated f h0 h1 (LSeq.create 12 (u64 0)))
 
 
 val make_base_point: p:point -> Stack unit
   (requires fun h -> live h p)
   (ensures fun h0 _ h1 -> modifies (loc p) h0 h1 /\
-    point_inv h1 p /\
-    (let (px, py, pz) = as_point_nat h1 p in
-    SM.fromDomain_ px == S.g_x /\
-    SM.fromDomain_ py == S.g_y /\
-    SM.fromDomain_ pz == 1))
+    point_inv h1 p /\ SM.fromDomainPoint (as_point_nat h1 p) == S.base_point)
 
 
 val make_point_at_inf: p:point -> Stack unit
   (requires fun h -> live h p)
   (ensures fun h0 _ h1 -> modifies (loc p) h0 h1 /\
-    point_inv h1 p /\
-    (let (px, py, pz) = as_point_nat h1 p in
-    SM.fromDomain_ px == 0 /\
-    SM.fromDomain_ py == 0 /\
-    SM.fromDomain_ pz == 0))
+    point_inv h1 p /\ SM.fromDomainPoint (as_point_nat h1 p) == S.point_at_inf)
 
 
 inline_for_extraction noextract
@@ -144,6 +147,23 @@ val copy_point: p:point -> res:point -> Stack unit
   (requires fun h -> live h p /\ live h res /\ disjoint p res)
   (ensures fun h0 _ h1 -> modifies (loc res) h0 h1 /\
     as_seq h1 res == as_seq h0 p)
+
+
+///  check if a point is a point-at-infinity
+
+val is_point_at_inf: p:point -> Stack uint64
+  (requires fun h -> live h p /\ point_inv h p)
+  (ensures fun h0 r h1 -> modifies0 h0 h1 /\
+    (if S.is_point_at_inf (SM.fromDomainPoint (as_point_nat h0 p))
+     then v r = ones_v U64 else v r = 0) /\
+    (if S.is_point_at_inf (as_point_nat h0 p)
+     then v r = ones_v U64 else v r = 0))
+
+
+val is_point_at_inf_vartime: p:point -> Stack bool
+  (requires fun h -> live h p /\ point_inv h p)
+  (ensures  fun h0 r h1 -> modifies0 h0 h1 /\
+    r == S.is_point_at_inf (as_point_nat h0 p))
 
 
 ///  Point conversion between Montgomery and Regular representations
@@ -173,24 +193,6 @@ val point_from_mont: p:point -> res:point-> Stack unit
     rx == SM.fromDomain_ px /\
     ry == SM.fromDomain_ py /\
     rz == SM.fromDomain_ pz))
-
-
-///  check if a point is a point-at-infinity
-
-val is_point_at_inf: p:point -> Stack uint64
-  (requires fun h -> live h p /\ point_inv h p)
-  (ensures fun h0 r h1 -> modifies0 h0 h1 /\
-    ((v r == 0 \/ v r == ones_v U64) /\
-    (if S.is_point_at_inf (SM.fromDomainPoint (as_point_nat h0 p))
-     then v r = ones_v U64 else v r = 0) /\
-    (if S.is_point_at_inf (as_point_nat h0 p)
-     then v r = ones_v U64 else v r = 0)))
-
-
-val is_point_at_inf_vartime: p:point -> Stack bool
-  (requires fun h -> live h p /\ point_inv h p)
-  (ensures  fun h0 r h1 -> modifies0 h0 h1 /\
-    r == S.is_point_at_inf (as_point_nat h0 p))
 
 
 ///  Point conversion between Jacobian and Affine coordinates representations
@@ -230,6 +232,8 @@ val is_point_on_curve_vartime: p:aff_point -> Stack bool
     r == S.is_point_on_curve (as_aff_point_nat h0 p))
 
 
+///  Point load and store functions
+
 val aff_store_point: res:lbuffer uint8 64ul -> p:aff_point -> Stack unit
   (requires fun h ->
     live h res /\ live h p /\ disjoint res p /\
@@ -247,6 +251,17 @@ val load_point_vartime: p:point -> b:lbuffer uint8 64ul -> Stack bool
       as_point_nat h1 p == Some?.v ps))))
 
 
+val aff_point_decompress_vartime (x y:felem) (s:lbuffer uint8 33ul) : Stack bool
+  (requires fun h ->
+    live h x /\ live h y /\ live h s /\
+    disjoint x y /\ disjoint x s /\ disjoint y s)
+  (ensures fun h0 b h1 -> modifies (loc x |+| loc y) h0 h1 /\
+    (b <==> Some? (S.aff_point_decompress (as_seq h0 s))) /\
+    (b ==> (let (xa, ya) = Some?.v (S.aff_point_decompress (as_seq h0 s)) in
+    as_nat h1 x < S.prime /\ as_nat h1 y < S.prime /\ as_nat h1 x == xa /\ as_nat h1 y == ya)))
+
+
+
 // TODO: mv
 inline_for_extraction noextract
 val validate_pubkey: pk:lbuffer uint8 64ul -> Stack bool
@@ -261,13 +276,3 @@ val isMoreThanZeroLessThanOrder: x:lbuffer uint8 32ul -> Stack bool
   (ensures  fun h0 r h1 -> modifies0 h0 h1 /\
     (let scalar = BSeq.nat_from_bytes_be (as_seq h0 x) in
     r <==> (0 < scalar && scalar < S.order)))
-
-
-val aff_point_decompress_vartime (x y:felem) (s:lbuffer uint8 33ul) : Stack bool
-  (requires fun h ->
-    live h x /\ live h y /\ live h s /\
-    disjoint x y /\ disjoint x s /\ disjoint y s)
-  (ensures fun h0 b h1 -> modifies (loc x |+| loc y) h0 h1 /\
-    (b <==> Some? (S.aff_point_decompress (as_seq h0 s))) /\
-    (b ==> (let (xa, ya) = Some?.v (S.aff_point_decompress (as_seq h0 s)) in
-    as_nat h1 x < S.prime /\ as_nat h1 y < S.prime /\ as_nat h1 x == xa /\ as_nat h1 y == ya)))
